renaming: ChangePartition -> Relabel

theories/TM/Combinators/Combinators.v
@@ -20,18 +20,18 @@ End Id.
 
 
 (** Simple operator to change the partition *)
-Section ChangePartition.
+Section Relabel.
   Variable (sig : finType) (n : nat).
   Variable F F' : finType.
   Variable pM : { M : mTM sig n & states M -> F }.
   Variable p : F -> F'.
 
-  Definition ChangePartition : { M : mTM sig n & states M -> F' } :=
+  Definition Relabel : { M : mTM sig n & states M -> F' } :=
     (projT1 pM; fun q => p (projT2 pM q)).
 
-  Lemma ChangePartition_Realise R :
+  Lemma Relabel_Realise R :
     pM ⊨ R ->
-    ChangePartition ⊨ ⋃_y (R |_ y) ||_(p y).
+    Relabel ⊨ ⋃_y (R |_ y) ||_(p y).
   Proof.
     intros HRel.
     intros tin k outc HLoop.
@@ -39,19 +39,19 @@ Section ChangePartition.
     hnf. exists (projT2 pM (cstate outc)). hnf. cbn. auto.
   Qed.
 
-  Lemma ChangePartition_RealiseIn R k :
+  Lemma Relabel_RealiseIn R k :
     pM ⊨c(k) R ->
-    ChangePartition ⊨c(k) ⋃_y (R |_ y) ||_(p y).
+    Relabel ⊨c(k) ⋃_y (R |_ y) ||_(p y).
   Proof. firstorder. Qed.
 
-  Lemma ChangePartition_Terminates T :
+  Lemma Relabel_Terminates T :
     projT1 pM ↓ T ->
-    projT1 ChangePartition ↓ T.
+    projT1 Relabel ↓ T.
   Proof. firstorder. Qed.
 
-End ChangePartition.
+End Relabel.
 
-Arguments ChangePartition : simpl never.
+Arguments Relabel : simpl never.
 
 
 (** Special case of the above operator, where we just fix a partitioparametern *)
@@ -63,7 +63,7 @@ Section Return.
   Variable F' : finType.
   Variable p : F'.
 
-  Definition Return := ChangePartition pM (fun _ => p).
+  Definition Return := Relabel pM (fun _ => p).
 
   Lemma Return_Realise R :
     pM ⊨ R ->
@@ -199,9 +199,9 @@ Ltac smpl_TM_Combinators :=
   | [ |- projT1 (Seq _ _) ↓ _] => eapply Seq_TerminatesIn
   | [ |- While _ ⊨ _] => eapply While_Realise
   | [ |- projT1 (While _) ↓ _] => eapply While_TerminatesIn
-  | [ |- ChangePartition _ _ ⊨ _] => eapply ChangePartition_Realise
-  | [ |- ChangePartition _ _ ⊨c(_) _] => eapply ChangePartition_RealiseIn
-  | [ |- projT1 (ChangePartition _ _) ↓ _] => eapply ChangePartition_Terminates
+  | [ |- Relabel _ _ ⊨ _] => eapply Relabel_Realise
+  | [ |- Relabel _ _ ⊨c(_) _] => eapply Relabel_RealiseIn
+  | [ |- projT1 (Relabel _ _) ↓ _] => eapply Relabel_Terminates
   | [ |- Return _ _ ⊨ _] => eapply Return_Realise
   | [ |- Return _ _ ⊨c(_) _] => eapply Return_RealiseIn
   | [ |- projT1 (Return _ _) ↓ _] => eapply Return_Terminates
